update point to resource

clightlight/Clight_Mem1.v
@@ -8,13 +8,13 @@ Require Import PCM.
 Require Import HoareDef STB.
 Require Import ProofMode.
 Require Import Any.
-From compcert Require Import Ctypes Floats Integers Values Memory AST.
+From compcert Require Import Ctypes Floats Integers Values Memory AST Clight.
 
 Set Implicit Arguments.
 
 
-Let _memcntRA: URA.t := (block ==> Z ==> (Excl.t memval))%ra.
-Let _memszRA: URA.t := (block ==> (Excl.t nat))%ra.
+Let _memcntRA: URA.t := (block ==> Z ==> (Consent.t memval))%ra.
+Let _memszRA: URA.t := (block ==> (Excl.t Z))%ra.
 
 Compute (URA.car (t:=_memcntRA)).
 Compute (URA.car (t:=_memszRA)).
@@ -27,9 +27,14 @@ Section POINTSTO.
 
   Local Open Scope Z.
 
-  Definition __points_to (b: block) (ofs: Z) (vs: list memval): _memcntRA :=
-    (fun _b _ofs => if (dec _b b) && ((ofs <=? _ofs) && (_ofs <? (ofs + Z.of_nat (List.length vs))))
-                    then (List.nth_error vs (Z.to_nat (_ofs - ofs))) else ε)
+  Definition __points_to (b: block) (ofs: Z) (q: Qnn) (mvs: list memval): _memcntRA :=
+    (fun _b _ofs => if (dec _b b) && ((ofs <=? _ofs) && (_ofs <? (ofs + Z.of_nat (List.length mvs))))
+                    then 
+                      match List.nth_error mvs (Z.to_nat (_ofs - ofs)) with
+                      | Some mv => Consent.just q mv
+                      | None => ε
+                      end
+                    else ε)
   .
 
   (* Opaque _points_to. *)
@@ -40,12 +45,12 @@ Section POINTSTO.
   .
   Proof. refl. Qed. *)
 
-  Definition _points_to (b: block) (ofs: Z) (vs: list memval): memcntRA := Auth.white (__points_to b ofs vs).
+  Definition _points_to (b: block) (ofs: Z) (q: Qnn) (mvs: list memval): memcntRA := Auth.white (__points_to b ofs q mvs).
 
   Lemma _points_to_split_aux
-        blk ofs hd tl
+        blk ofs hd tl q
     :
-      (_points_to blk ofs (hd :: tl)) = (_points_to blk ofs [hd]) ⋅ (_points_to blk (ofs + 1)%Z tl)
+      (_points_to blk ofs q (hd :: tl)) = (_points_to blk ofs q [hd]) ⋅ (_points_to blk (ofs + 1)%Z q tl)
   .
   Proof.
     ss. unfold _points_to, Auth.white. repeat (rewrite URA.unfold_add; ss).
@@ -55,42 +60,41 @@ Section POINTSTO.
       try rewrite Z.leb_gt in *; try rewrite Z.leb_le in *; try rewrite Z.ltb_ge in *; try rewrite Z.ltb_lt in *; try lia; clarify.
     - clear_tac. subst. rewrite Zpos_P_of_succ_nat in *. rewrite <- Zlength_correct in *.
       assert(x0 = ofs). { lia. } subst.
-      rewrite Z.sub_diag in *. ss.
+      rewrite Z.sub_diag in *. ss. clarify. 
     - clear_tac. rewrite Zpos_P_of_succ_nat in *. rewrite <- Zlength_correct in *.
       destruct (Z.to_nat (x0 - ofs)) eqn:T; ss.
       { exfalso. lia. }
-      rewrite Z.sub_add_distr in *. rewrite Z2Nat.inj_sub in Heq1; ss. rewrite T in *. ss. rewrite Nat.sub_0_r in *. ss.
+      rewrite Z.sub_add_distr in *. rewrite Z2Nat.inj_sub in Heq4; ss. rewrite T in *. ss. rewrite Nat.sub_0_r in *. ss. clarify.
     - clear_tac. rewrite Zpos_P_of_succ_nat in *. rewrite <- Zlength_correct in *.
       destruct (Z.to_nat (x0 - ofs)) eqn:T; ss.
       { exfalso. lia. }
-      rewrite Z.sub_add_distr in *. rewrite Z2Nat.inj_sub in Heq1; ss. rewrite T in *. ss. rewrite Nat.sub_0_r in *. ss.
+      rewrite Z.sub_add_distr in *. rewrite Z2Nat.inj_sub in Heq4; ss. rewrite T in *. ss. rewrite Nat.sub_0_r in *. ss. clarify.
     - clear_tac. rewrite Zpos_P_of_succ_nat in *. rewrite <- Zlength_correct in *.
       assert(x0 = ofs). { lia. } subst.
       rewrite Z.sub_diag in *. ss.
     - clear_tac. rewrite Zpos_P_of_succ_nat in *. rewrite <- Zlength_correct in *.
       destruct (Z.to_nat (x0 - ofs)) eqn:T; ss.
       { exfalso. lia. }
-      rewrite Z.sub_add_distr in *. rewrite Z2Nat.inj_sub in Heq1; ss. rewrite T in *. ss. rewrite Nat.sub_0_r in *. ss.
     - clear_tac. rewrite Zpos_P_of_succ_nat in *. rewrite <- Zlength_correct in *.
-      assert(x0 = ofs). { lia. } subst.
-      rewrite Z.sub_diag in *. ss.
+      destruct (Z.to_nat (x0 - ofs)) eqn:T; ss.
+      rewrite Z.sub_add_distr in *. rewrite Z2Nat.inj_sub in Heq4; ss. rewrite T in *. ss. rewrite Nat.sub_0_r in *. ss. clarify.
   Qed.
 
-  Lemma __points_to_nil : forall blk ofs _b _ofs, __points_to blk ofs [] _b _ofs = ε.
+  Lemma __points_to_nil : forall blk ofs q _b _ofs, __points_to blk ofs q [] _b _ofs = ε.
   Proof.
     intros. unfold __points_to. ss. destruct ((ofs <=? _ofs) && (_ofs <? ofs + 0)) eqn : E; try nia.
     bsimpl. auto.
   Qed.
 
-  Lemma points_to_nil : forall blk ofs, _points_to blk ofs [] = ε.
+  Lemma points_to_nil : forall blk ofs q, _points_to blk ofs q [] = ε.
   Proof.
     intros. ss. unfold _points_to, Auth.white.
     change (memcntRA.(URA.unit)) with (Auth.frag (_memcntRA.(URA.unit))). f_equal. ss.
     repeat (apply func_ext; i). apply __points_to_nil.
   Qed.
 
-  Lemma _points_to_app l l' blk ofs:
-    (_points_to blk ofs (l++l')) = (_points_to blk ofs l) ⋅ (_points_to blk (ofs + length l) l').
+  Lemma _points_to_app l l' q blk ofs:
+    (_points_to blk ofs q (l++l')) = (_points_to blk ofs q l) ⋅ (_points_to blk (ofs + length l) q l').
   Proof.
     revert l' blk ofs. induction l;i;ss.
     - rewrite points_to_nil. rewrite URA.unit_idl. rewrite Z.add_0_r. auto.
@@ -101,9 +105,9 @@ Section POINTSTO.
   Qed.
 
   Lemma _points_to_split :
-    forall (blk : Values.block) (ofs : Z) (n : nat) (l : list memval),
-      _points_to blk ofs l =
-        _points_to blk ofs (firstn n l) ⋅ _points_to blk (ofs + (length (firstn n l))) (skipn n l).
+    forall (blk : Values.block) (ofs : Z) (q: Qnn) (n : nat) (l : list memval),
+      _points_to blk ofs q l =
+        _points_to blk ofs q (firstn n l) ⋅ _points_to blk (ofs + (length (firstn n l))) q (skipn n l).
   Proof.
     intros. set l as k at 2 3 4. rewrite <- (firstn_skipn n l). unfold k. clear k.
     rewrite _points_to_app. auto.
@@ -113,27 +117,15 @@ End POINTSTO.
 
 Section SZOF.
 
-  Definition __sz_of (b: block) (sz: nat) : _memszRA :=
+  Definition __sz_of (b: block) (sz: Z) : _memszRA :=
     (fun _b => if dec _b b
                then Excl.just sz
                else ε)
   .
 
-  Definition _sz_of (b: block) (sz: nat) : memszRA := Auth.white (__sz_of b sz).
+  Definition _sz_of (b: block) (sz: Z) : memszRA := Auth.white (__sz_of b sz).
 
 End SZOF.
-  
-  (** TODO-var **)
-  (* Definition initial_mem_mr (csl: gname -> bool) (sk: Sk.t): _memRA := *)
-  (*   fun blk ofs => *)
-  (*     match List.nth_error sk (Pos.to_nat blk) with *)
-  (*     | Some (g, gd) => *)
-  (*       match gd with *)
-  (*       | Sk.Gfun => ε *)
-  (*       | Sk.Gvar gv => if csl g then if (dec ofs 0%Z) then Some (Vint (Int.repr gv)) else ε else ε *)
-  (*       end *)
-  (*     | _ => ε *)
-  (*     end. *)
 
 End RA.
 
@@ -150,24 +142,42 @@ Section PROP.
     unfold updblk, getblk. rewrite <- drop_drop. do 2 rewrite firstn_skipn. refl.
   Qed.
 
-  Definition points_to addr vs : iProp :=
-    match addr with
-    | Vptr b ofs => OwnM (_points_to b (Ptrofs.unsigned ofs) vs)
-    | _ => ⌜False⌝
-    end.
+  Definition size_rule (sz: nat) : Z :=
+    if sz <? 2 then 1
+    else if sz <? 4 then 2
+    else if sz <? 8 then 4
+    else 8
+  .
 
-  Definition mpoints_to addr sz vs : iProp :=
+  Definition points_to addr q mvs : iProp :=
     match addr with
     | Vptr b ofs =>
-        OwnM (_points_to b (Ptrofs.unsigned ofs) vs)
-        ** OwnM (_sz_of b sz)
-    | _ => ⌜False⌝
+          let ofs' := Ptrofs.unsigned ofs in
+          let align := size_rule (Z.to_nat (length mvs)) in
+          OwnM (_points_to b ofs' q mvs)
+          ** ⌜(align | ofs')⌝
+    | _ => ⌜False⌝%I 
     end.
 
-  Notation "addr ↦ vs" := (points_to addr vs) (at level 20).
-  Notation "addr #↦ vs ⋯ sz" := (mpoints_to addr sz vs) (at level 10).
+  Definition mpoints_to addr sz mvs : iProp :=
+    match addr with
+    | Vptr b ofs =>
+          let ofs' := Ptrofs.unsigned ofs in
+          let align := size_rule (Z.to_nat sz) in
+          OwnM (_points_to b ofs' 1 mvs) ** OwnM (_sz_of b sz)
+          ** ⌜(align | ofs')⌝
+    | _ => ⌜False⌝%I 
+    end.
 
-  Lemma detach_size addr vs sz : (addr #↦ vs ⋯ sz) -∗ (addr ↦ vs).
+  Definition has_addr v b ofs : iProp :=
+    match v with
+    | Vptr b' ofs' => ⌜b' = b /\ Ptrofs.unsigned ofs' = ofs⌝%I
+    | _ => ⌜False⌝%I 
+    end.
+
+  Definition allocated b sz : iProp := OwnM (_sz_of b sz).
+
+  (* Lemma detach_size addr vs sz : (addr #↦ vs ⋯ sz) -∗ (addr ↦ vs).
   Proof. 
     iIntros "A". unfold mpoints_to, points_to. des_ifs.
     iDestruct "A" as "[B C]". iApply "B".
@@ -208,16 +218,18 @@ Section PROP.
     iSplitL "B";auto. iIntros "B". iCombine "B C" as "B". rewrite <- _points_to_split.
     iCombine "A B" as "A". replace (ofs + m) with (ofs + Z.to_nat m) by nia.
     rewrite <- _points_to_split';auto.
-  Qed.
+  Qed. *)
 
 End PROP.
 
+Notation "addr ↦ ( q , mvs )" := (points_to addr q mvs) (at level 20).
+Notation "addr #↦ vs ⋯ sz" := (mpoints_to addr sz vs) (at level 10).
 
 Section AUX.
 
   Context `{@GRA.inG memRA Σ}.
 
-  Lemma points_to_disj
+  (* Lemma points_to_disj
         ptr x0 x1
     :
       (ptr |-> [x0] -∗ ptr |-> [x1] -* ⌜False⌝)
@@ -227,7 +239,7 @@ Section AUX.
     iIntros "A B". iCombine "A B" as "A". iOwnWf "A" as WF0.
     unfold _points_to in WF0. rewrite ! unfold__points_to in *. repeat (ur in WF0); ss.
     specialize (WF0 blk ofs). des_ifs; bsimpl; des; SimComp.Coqlib.des_sumbool; zsimpl; ss; try lia.
-  Qed.
+  Qed. *)
 
   (** TODO-is_list **)
   (* Fixpoint is_list (ll: val) (xs: list val): iProp := *)
@@ -273,11 +285,11 @@ Section AUX.
   (* Qed. *)
 
   (* Global Opaque is_list. *)
-  Definition encode_list chunk vlist : list memval := flat_map (encode_val chunk) vlist. 
+  (* Definition encode_list chunk vlist : list memval := flat_map (encode_val chunk) vlist. 
   
   Definition is_arr (chunk : memory_chunk) (ll : val) (xs : list val) :=
     (∃ (b :block) (ofs : ptrofs),
-        ⌜ll = Vptr b ofs⌝ ** (b, Ptrofs.intval ofs) |-> (encode_list chunk xs))%I.
+        ⌜ll = Vptr b ofs⌝ ** (b, Ptrofs.intval ofs) |-> (encode_list chunk xs))%I. *)
 End AUX.
 
 Definition wordsize_64 := 64%nat.
@@ -296,163 +308,130 @@ Ltac unfold_intrange_64 := unfold intrange_64, min_64, max_64 in *; unfold modul
 Ltac unfold_modrange_64 := unfold modrange_64, modulus_64, wordsize_64 in *.
 
 Section PROOF.
-  Context `{@GRA.inG memRA Σ}.
 
- Definition alloc_spec: fspec :=
-    (mk_simple (fun '(lo, hi) => (
+  Context `{@GRA.inG memcntRA Σ}.
+  Context `{@GRA.inG memszRA Σ}.
+  
+  Definition salloc_spec: fspec :=
+    (mk_simple (fun sz => (
                     (ord_pure 0%nat),
-                    (fun varg => (⌜varg = (lo, hi)↑ /\ (lo <= hi)%Z⌝)%I),
-                    (fun vret => (∃ b, (⌜vret = b↑⌝
-                                      ** ((b, lo) |-> (List.repeat Undef (Z.to_nat (hi - lo))))))%I
-    )))).
+                    (fun varg => ⌜varg = sz↑⌝),
+                    (fun vret => ∃ b addr, ⌜vret = b↑⌝
+                                 ** addr ↦ (1, List.repeat Undef (Z.to_nat sz))
+                                 ** has_addr addr b 0)
+    )))%I.
 
-  Definition free_spec: fspec :=
+  Definition sfree_spec: fspec :=
     (mk_simple (fun '() => (
                    (ord_pure 0%nat),
-                   (fun varg => (∃ l b lo hi, (⌜varg = (b, lo, hi)↑ /\ Z.of_nat (List.length l) = hi - lo⌝) ** ((b, lo) |-> l))%I),
-                    fun vret => ⌜vret = tt↑⌝%I
-    ))).
+                   (fun varg => ∃ mvl addr b sz, ⌜varg = (b, sz)↑ /\ Z.of_nat (List.length mvl) = sz⌝
+                                ** addr ↦ (1, mvl)
+                                ** has_addr addr b 0),
+                   (fun vret => ⌜vret = tt↑⌝)
+    )))%I.
 
   Definition load_spec: fspec :=
-    (mk_simple (fun '(chunk, b, ofs, l) => (
+    (mk_simple (fun '(chunk, addr, q, l) => (
                     (ord_pure 0%nat),
-                    (fun varg => (⌜varg = (chunk, b, Ptrofs.repr ofs)↑⌝) ** ((b, ofs) |-> l)),
-                    (fun vret => (∃ v, (b, ofs) |-> l ** ⌜vret = v↑ /\ decode_val chunk l = v⌝)%I)
-    ))).
+                    (fun varg => ⌜varg = (chunk, addr)↑ /\ (0 ≤ q)%Qnn ⌝ ** addr ↦ (q, l)),
+                    (fun vret => ∃ v, ⌜vret = v↑ /\ decode_val chunk l = v⌝ ** addr ↦ (q, l))
+    )))%I.
 
   Definition loadbytes_spec: fspec :=
-    (mk_simple (fun '(b, ofs, n, l) => (
+    (mk_simple (fun '(addr, q, n, l) => (
                     (ord_pure 0%nat),
-                    (fun varg => (⌜varg = (b, Ptrofs.repr ofs, n)↑ /\ (Z.of_nat (List.length l) = n)⌝) ** (((b, ofs) |-> l))),
-                    (fun vret => ((b, ofs) |-> l) ** ⌜vret = l↑⌝)
+                    (fun varg => ⌜varg = (addr, n)↑ /\ Z.of_nat (List.length l) = n /\ (0 ≤ q)%Qnn⌝ ** addr ↦ (q, l)),
+                    (fun vret => ⌜vret = l↑⌝ ** addr ↦ (q, l))
     ))).
 
   Definition store_spec: fspec :=
     (mk_simple
-       (fun '(chunk, b, ofs, v_new) => (
+       (fun '(chunk, addr, v_new) => (
             (ord_pure 0%nat),
-            (fun varg => (∃ l_old, (⌜varg = (chunk, b, Ptrofs.repr ofs, v_new)↑ /\ List.length l_old = size_chunk_nat chunk⌝) ** ((b, ofs) |-> l_old))%I),
-            (fun vret => (∃ l_new, ((b, ofs) |-> l_new) ** ⌜vret = tt↑ /\ encode_val chunk v_new = l_new⌝)%I)
-    ))).
+            (fun varg => ∃ l_old, ⌜varg = (chunk, addr, v_new)↑ /\ List.length l_old = size_chunk_nat chunk⌝
+                         ** addr ↦ (1, l_old)),
+            (fun vret => ∃ l_new, ⌜vret = tt↑ /\ encode_val chunk v_new = l_new⌝
+                         ** addr ↦ (1, l_new))
+    )))%I.
 
   Definition storebytes_spec: fspec :=
     (mk_simple
-       (fun '(b, ofs, l_new) => (
+       (fun '(addr, l_new) => (
             (ord_pure 0%nat),
-            (fun varg => (∃ l_old, (⌜varg = (b, ofs, l_new)↑ /\ List.length l_old = List.length l_new⌝) ** ((b, ofs) |-> l_old))%I),
-            (fun vret => ((b, ofs) |-> l_new) ** ⌜vret = tt↑⌝)
-    ))).
+            (fun varg => ∃ l_old, ⌜varg = (addr, l_new)↑ /\ List.length l_old = List.length l_new⌝
+                         ** addr ↦ (1, l_old)),
+            (fun vret => ⌜vret = tt↑⌝ ** addr ↦ (1, l_new))
+    )))%I.
 
   Definition valid_pointer_spec: fspec :=
     (mk_simple
-       (fun '(result, resource) => (
+       (fun '(result, iprop) => (
             (ord_pure 0%nat),
             (fun varg =>
-               ((∃ b ofs v, ⌜varg = (b, ofs)↑⌝ ** ⌜resource = (_points_to (b, ofs) [v])⌝ ** ⌜result = true⌝) ∨
-                (∃ b ofs v, ⌜varg = (b, ofs)↑⌝ ** ⌜resource <> (_points_to (b, ofs) [v])⌝ ** ⌜result = false⌝))
-                 ** OwnM (resource)
-            ),
-            (fun vret => OwnM(resource) ** ⌜vret = result↑⌝)
-    ))).
+            ((∃ addr q mvl, ⌜varg = addr↑ /\ iprop = (addr ↦ (q, mvl)) /\ result = true⌝) ∨
+                (∃ addr q mvl, ⌜varg = addr↑ /\ iprop <> (addr ↦ (q, mvl)) /\ result = false⌝))
+                ** iprop),
+            (fun vret => ⌜vret = result↑⌝ ** iprop)%I
+    )))%I.
 
-  (* about capture *)
-  
-  (* { True } capture(p) { exists v, v.p ~ v } *)
-  (* { p ~ v } (int)(p) { v } -> all pointer to int casting in C became capture and assign. *)
-  (* { (p |-> _) * p ~ i } (ptr)i { r. r = p } *)
-
-  (* p ~ i0 /\ p ~ i1 -> i0 = i1 *)
-  (* p ~ i  ->  p+j ~ i+j *)
-
-  (* p ~ i -> p~i * p~i *)
-
-  Context `{@GRA.inG memRACAP Σ}.
-
-  Definition capture_spec: fspec :=
-    (@mk_simple _ (block * ptrofs)
-       (fun '(b, ofs) => (
-            (ord_pure 0%nat),
-            (fun varg:Any.t => @bi_pure iProp (varg = (b, ofs)↑)),
-            (fun vret => (∃ addr, ((b, Ptrofs.signed ofs) ~~ Ptrofs.signed addr) ** ⌜vret = addr↑⌝)%I)
-    ))).
-
-  (* Set Printing All. *)
-  Definition int2ptr_spec: fspec :=
-    (mk_simple
-       (fun '(b, ofs) => (
-            (ord_pure 0%nat),
-            (fun varg:Any.t =>
-               (∃ addr l, (⌜varg = addr↑⌝) ** ((b, ofs) ~~ addr) ** ((b, ofs) |-> l))%I
-            ),
-            (fun vret => (⌜vret = (b, ofs)↑⌝)%I)
-    ))).
-
-  (* Set Printing All. *)
-  Definition ptr2int_spec: fspec :=
-    (mk_simple
-       (fun '(addr) => (
-            (ord_pure 0%nat),
-            (fun varg:Any.t =>
-               (∃ b ofs, (⌜varg = (b, ofs)↑⌝) ** ((b, ofs) ~~ addr))%I
-            ),
-            (fun vret => (⌜vret = addr↑⌝)%I)
-    ))).
-
-  Context `{@GRA.inG memRASZ Σ}.
-
+  (* heap malloc free *)
   Definition malloc_spec: fspec :=
     (mk_simple (fun sz => (
                     (ord_pure 0%nat),
-                    (fun varg => (⌜varg = (Vint (Int.repr (Z.of_nat sz)))↑ /\ (8 * (Z.of_nat sz) < modulus_64)%Z⌝: iProp)%I),
-                    (fun vret => (∃ b, (⌜vret = (Vptr b (Ptrofs.repr 0))↑⌝)
-                                      ** ((b, 0%Z) |-> (List.repeat Undef sz))
-                                      ** ((b, 0%Z) :== sz)): iProp)%I
-    ))).
+                    (fun varg => ⌜varg = (Vptrofs sz)↑⌝),
+                    (fun vret => ∃ addr b, ⌜vret = addr↑⌝
+                                 ** addr #↦ List.repeat Undef (Z.to_nat (Ptrofs.unsigned sz)) ⋯ (Ptrofs.unsigned sz)
+                                 ** has_addr addr b 0) 
+    )))%I.
 
-  (* malloc free *)
   Definition mfree_spec: fspec :=
-    (mk_simple (fun '(b, ofs) => (
+    (mk_simple (fun '() => (
                     (ord_pure 0%nat),
-                    (fun varg => (∃ l sz, (⌜varg = (b, ofs)↑ /\ Z.of_nat (List.length l) = sz⌝)
-                                         ** ((b, ofs) |-> l)
-                                         ** ((b, ofs) :== sz)
-                              )%I),
-                    fun vret => ⌜vret = tt↑⌝%I
-    ))).
+                    (fun varg => ∃ mvl addr b sz, ⌜varg = addr↑ /\ Z.of_nat (List.length mvl) = sz⌝
+                                 ** addr #↦ mvl ⋯ sz
+                                 ** has_addr addr b 0),
+                    (fun vret => ⌜vret = tt↑⌝)
+    )))%I.
 
   
   Definition MemStb: list (gname * fspec).
     eapply (Seal.sealing "stb").
-    apply [("alloc", alloc_spec); ("free", free_spec); ("load", load_spec);
-           ("loadbytes", loadbytes_spec); ("store", store_spec); ("storebytes", storebytes_spec);
-           ("valid_pointer", valid_pointer_spec); ("capture", capture_spec); ("int2ptr", int2ptr_spec);
-           ("ptr2int", ptr2int_spec); ("malloc", malloc_spec); ("mfree", mfree_spec)
-      ].
-  Defined.
+    apply [("salloc", salloc_spec); ("sfree", sfree_spec); 
+           ("load", load_spec); ("loadbytes", loadbytes_spec); 
+           ("store", store_spec); ("storebytes", storebytes_spec);
+           ("valid_pointer", valid_pointer_spec);
+           ("malloc", malloc_spec); ("mfree", mfree_spec)
+           ].
+    Defined.
 
   Definition MemSbtb: list (gname * fspecbody) :=
-    [("alloc", mk_specbody alloc_spec (fun _ => trigger (Choose _)));
-    ("free",   mk_specbody free_spec (fun _ => trigger (Choose _)));
+    [("salloc", mk_specbody salloc_spec (fun _ => trigger (Choose _)));
+    ("sfree",   mk_specbody sfree_spec (fun _ => trigger (Choose _)));
     ("load",   mk_specbody load_spec (fun _ => trigger (Choose _)));
     ("loadbytes",   mk_specbody loadbytes_spec (fun _ => trigger (Choose _)));
     ("store",  mk_specbody store_spec (fun _ => trigger (Choose _)));
     ("storebytes",   mk_specbody storebytes_spec (fun _ => trigger (Choose _)));
     ("valid_pointer",   mk_specbody valid_pointer_spec (fun _ => trigger (Choose _)));
-    ("capture",   mk_specbody capture_spec (fun _ => trigger (Choose _)));
-    ("int2ptr",   mk_specbody int2ptr_spec (fun _ => trigger (Choose _)));
-    ("ptr2int",   mk_specbody ptr2int_spec (fun _ => trigger (Choose _)));
     ("malloc",   mk_specbody malloc_spec (fun _ => trigger (Choose _)));
     ("mfree",   mk_specbody mfree_spec (fun _ => trigger (Choose _)))
     ]
   .
 
-  Variable csl: gname -> bool.
+  Definition initial_memcnt (sk: Sk.t): _memcntRA :=
+     fun blk ofs =>
+       match List.nth_error sk (pred (Pos.to_nat blk)) with
+       | Some (_, a) =>
+          match Any.downcast a : option (globdef Clight.fundef type) with
+          | Some (Gvar gv) => if (dec ofs 0%Z) then Some (Vint (Int.repr gv)) else ε 
+          | _ => ε
+          end
+       | _ => ε
+       end.
 
   Definition SMemSem (sk: Sk.t): SModSem.t := {|
     SModSem.fnsems := MemSbtb;
     SModSem.mn := "Mem";
-    (* SModSem.initial_mr := (GRA.embed (Auth.black (initial_mem_mr csl sk))); *)
-    SModSem.initial_mr := (GRA.embed (Auth.black ε));
+    SModSem.initial_mr := (GRA.embed (Auth.black (initial_mem_mr csl sk))) ⋅ (GRA.embed (Auth.black _memszRA.(URA.unit)));
     SModSem.initial_st := tt↑;
   |}
   .
